src/ModSimNoSync.v
@@ -465,8 +465,10 @@ Section PRIMIVIESIM.
            tid ths1
            (THS: TIdSet.add_new tid ths0 ths1)
            (VALID: URA.wf (r_shared0 ⋅ r_ctx0)),
-    exists r_shared1 r_own,
-      (<<INV: I (ths1, im_src0, im_tgt0, st_src0, st_tgt0, r_shared1)>>) /\
+    forall im_tgt0'
+      (UPD: fair_update im_tgt0 im_tgt0' (sum_fmap_l (fun t => if (tid_dec t tid) then Flag.success else Flag.emp))),
+    exists r_shared1 r_own im_src0',
+      (<<INV: I (ths1, im_src0', im_tgt0', st_src0, st_tgt0, r_shared1)>>) /\
         (<<VALID: URA.wf (r_shared1 ⋅ r_own ⋅ r_ctx0)>>) /\
         (forall ths im_src1 im_tgt1 st_src st_tgt r_shared2 r_ctx2
                 (INV: I (ths, im_src1, im_tgt1, st_src, st_tgt, r_shared2))
