src/ModSimStid.v
@@ -485,8 +485,10 @@ Section PRIMIVIESIM.
            tid ths1
            (THS: TIdSet.add_new tid ths0 ths1)
            (VALID: URA.wf (r_shared0 ⋅ r_ctx0)),
-    exists r_shared1 r_own,
-      (<<INV: I (ths1, im_src0, im_tgt0, st_src0, st_tgt0, r_shared1)>>) /\
+    forall im_tgt0'
+      (UPD: fair_update im_tgt0 im_tgt0' (sum_fmap_l (fun t => if (tid_dec t tid) then Flag.success else Flag.emp))),
+    exists r_shared1 r_own im_src0',
+      (<<INV: I (ths1, im_src0', im_tgt0', st_src0, st_tgt0, r_shared1)>>) /\
         (<<VALID: URA.wf (r_shared1 ⋅ r_own ⋅ r_ctx0)>>) /\
         (forall ths im_src1 im_tgt1 st_src st_tgt r_shared2 r_ctx2
                 (INV: I (ths, im_src1, im_tgt1, st_src, st_tgt, r_shared2))
@@ -503,17 +505,6 @@ Section PRIMIVIESIM.
                     src tgt
                     (ths, im_src2, im_tgt2, st_src, st_tgt, r_shared2)
                     >>)).
-
-  Definition shared_rel_wf: Prop :=
-    forall ths im_src0 im_tgt0 st_src st_tgt r_shared0 r_ctx
-           (INV: I (ths, im_src0, im_tgt0, st_src, st_tgt, r_shared0))
-           (VALID: URA.wf (r_shared0 ⋅ r_ctx)),
-    forall im_tgt1
-           (TGT: fair_update im_tgt0 im_tgt1 (sum_fmap_l (tids_fmap_all ths))),
-    exists im_src1 r_shared1,
-      (<<SRC: fair_update im_src0 im_src1 (sum_fmap_l (tids_fmap_all ths))>>) /\
-        (<<INV: I (ths, im_src1, im_tgt1, st_src, st_tgt, r_shared1)>>) /\
-        (<<VALID: URA.wf (r_shared1 ⋅ r_ctx)>>).
 
 End PRIMIVIESIM.
 #[export] Hint Constructors __lsim: core.
