src/ModSimStutter.v
@@ -841,31 +841,6 @@ Section PRIMIVIESIM.
                              (ths, im_src2, im_tgt2, st_src, st_tgt, r_shared2)
                              >>)).
 
-  (* Definition local_sim {R0 R1} (RR: R0 -> R1 -> Prop) src tgt := *)
-  (*   forall ths0 im_src0 im_tgt0 st_src0 st_tgt0 r_shared0 r_ctx0 *)
-  (*     (INV: I (ths0, im_src0, im_tgt0, st_src0, st_tgt0, r_shared0)) *)
-  (*     tid ths1 *)
-  (*     (THS: TIdSet.add_new tid ths0 ths1) *)
-  (*     (VALID: URA.wf (r_shared0 ⋅ r_ctx0)), *)
-  (*   exists r_shared1 r_own o, *)
-  (*     (<<INV: I (ths1, im_src0, im_tgt0, st_src0, st_tgt0, r_shared1)>>) /\ *)
-  (*       (<<VALID: URA.wf (r_shared1 ⋅ r_own ⋅ r_ctx0)>>) /\ *)
-  (*       (forall ths im_src1 im_tgt1 st_src st_tgt r_shared2 r_ctx2 *)
-  (*          (INV: I (ths, im_src1, im_tgt1, st_src, st_tgt, r_shared2)) *)
-  (*          (VALID: URA.wf (r_shared2 ⋅ r_own ⋅ r_ctx2)) *)
-  (*          im_tgt2 *)
-  (*          (TGT: fair_update im_tgt1 im_tgt2 (sum_fmap_l (tids_fmap tid ths))), *)
-  (*         exists im_src2, (<<SRC: fair_update im_src1 im_src2 (sum_fmap_l (tids_fmap tid ths))>>) /\ *)
-  (*                      (<<LSIM: forall fs ft, *)
-  (*                          lsim *)
-  (*                            tid *)
-  (*                            (@local_RR R0 R1 RR tid) *)
-  (*                            fs ft *)
-  (*                            r_ctx2 *)
-  (*                            (o, src) tgt *)
-  (*                            (ths, im_src2, im_tgt2, st_src, st_tgt, r_shared2) *)
-  (*                            >>)). *)
-
 End PRIMIVIESIM.
 #[export] Hint Constructors __lsim: core.
 #[export] Hint Unfold lsim: core.
