src/Stid2NoSync.v
@@ -137,3 +137,31 @@ Section PROOF.
   Qed.
 
 End PROOF.
+
+Section MODSIM.
+
+  Lemma stid_implies_nosync_mod
+        md_src md_tgt
+        (MDSIM: ModSimStid.ModSim.mod_sim md_src md_tgt)
+    :
+    ModSimNoSync.ModSim.mod_sim md_src md_tgt.
+  Proof.
+    inv MDSIM.
+    set (_ident_src := Mod.ident md_src). set (_ident_tgt := Mod.ident md_tgt).
+    set (state_src := Mod.state md_src). set (state_tgt := Mod.state md_tgt).
+    set (srcE := ((@eventE _ident_src +' cE) +' sE state_src)).
+    set (tgtE := ((@eventE _ident_tgt +' cE) +' sE state_tgt)).
+    set (ident_src := @ident_src _ident_src).
+    set (ident_tgt := @ident_tgt _ident_tgt).
+    set (shared := (TIdSet.t * (@imap ident_src wf_src) * (@imap ident_tgt wf_tgt) * state_src * state_tgt * URA.car)%type).
+    econs; eauto.
+    i. specialize (funs fn args). des_ifs.
+    unfold ModSimStid.local_sim in funs.
+    ii. specialize (funs _ _ _ _ _ _ _ INV tid _ THS VALID _ UPD).
+    des. esplits; eauto.
+    i. specialize (funs1 _ _ _ _ _ _ _ INV1 VALID1 _ TGT).
+    des. esplits; eauto. i. specialize (LSIM fs ft).
+    eapply stid_implies_nosync in LSIM. apply LSIM.
+  Qed.
+
+End MODSIM.
